add more information to types

C0deine/Type/Typ.lean
@@ -2,41 +2,123 @@ import C0deine.Utils.Symbol
 
 namespace C0deine
 
+inductive Typ.Primitive
+| int
+| bool
+deriving DecidableEq, Inhabited, Hashable
+
 mutual
 inductive Typ
 | prim (prim : Typ.Primitive)
 | mem (mem : Typ.Memory)
 | void
 | alias (sym : Symbol)
-
-inductive Typ.Primitive
-| int
-| bool
+deriving Inhabited, Hashable
 
 inductive Typ.Memory
 | pointer (typ : Typ)
 | array (typ : Typ)
 | struct (sym : Symbol)
+deriving Inhabited, Hashable
 end
 
 namespace C0deine.Typ
 
-mutual
 def Primitive.toString : Typ.Primitive → String
   | .int  => "int"
   | .bool => "bool"
 instance : ToString Typ.Primitive where toString := Typ.Primitive.toString
 
+mutual
 def Memory.toString : Typ.Memory → String
   | .pointer (typ : Typ)   => s!"{Typ.toString typ} *"
   | .array (typ : Typ)     => s!"{Typ.toString typ}[]"
   | .struct (sym : Symbol) => s!"struct {sym}"
-instance : ToString Typ.Memory where toString := Typ.Memory.toString
 
-def Typ.toString : Typ → String
+def toString : Typ → String
   | .prim (prim : Typ.Primitive) => Typ.Primitive.toString prim
   | .mem (mem : Typ.Memory) => Typ.Memory.toString mem
   | .void => "void"
   | .alias (sym : Symbol) => s!"{sym}"
-instance : ToString Typ where toString := Typ.toString
 end
+
+instance : ToString Typ.Memory where toString := Typ.Memory.toString
+instance : ToString Typ where toString := Typ.toString
+
+mutual
+def Typ.Memory.deq (a b : Typ.Memory) : Decidable (a = b) :=
+  match a, b with
+  | .struct s1, .struct s2 =>
+    match decEq s1 s2 with
+    | isTrue h  => isTrue  <| h ▸ rfl
+    | isFalse h => isFalse <| fun h' => by simp at h'; apply h h'
+  | .pointer t1, .pointer t2 =>
+    match Typ.deq t1 t2 with
+    | isTrue h  => isTrue  <| h ▸ rfl
+    | isFalse h => isFalse <| fun h' => by simp at h'; apply h h'
+  | .array t1, .array t2 =>
+    match Typ.deq t1 t2 with
+    | isTrue h  => isTrue  <| h ▸ rfl
+    | isFalse h => isFalse <| fun h' => by simp at h'; apply h h'
+  | _, _ => sorry
+    -- isFalse <| _
+
+def Typ.deq (a b : Typ) : Decidable (a = b) :=
+  match a, b with
+  | .prim p1, .prim p2 =>
+    match decEq p1 p2 with
+    | isTrue h  => isTrue  <| h ▸ rfl
+    | isFalse h => isFalse <| fun h' => by simp at h'; apply h h'
+  | .mem m1, .mem m2 =>
+    match Typ.Memory.deq m1 m2 with
+    | isTrue h  => isTrue  <| h ▸ rfl
+    | isFalse h => isFalse <| fun h' => by simp at h'; apply h h'
+  | .void, .void =>
+    isTrue <| Eq.refl Typ.void
+  | .alias s1, .alias s2 =>
+    match decEq s1 s2 with
+    | isTrue h  => isTrue  <| h ▸ rfl
+    | isFalse h => isFalse <| fun h' => by simp at h'; apply h h'
+  | _, _ => sorry
+    -- isFalse <| fun h => _
+
+end
+
+instance : DecidableEq Typ.Memory := Typ.Memory.deq
+instance : DecidableEq Typ := Typ.deq
+
+-- A type is reduced if it contains no aliases
+-- todo: do we need to lookup the symbol for structures?
+mutual
+inductive Reduced : Typ → Prop where
+| prim_int_reduced : Reduced (Typ.prim Typ.Primitive.int)
+| prim_bool_reduced : Reduced (Typ.prim Typ.Primitive.bool)
+| mem_reduced : ∀ m, Memory.Reduced m → Reduced (Typ.mem m)
+| void_reduced : Reduced Typ.void
+
+inductive Memory.Reduced : Memory → Prop where
+| pointer_reduced : ∀ t, Reduced t → Memory.Reduced (Typ.Memory.pointer t)
+| array_reduced   : ∀ t, Reduced t → Memory.Reduced (Typ.Memory.array t)
+| struct_reduced  : ∀ s, Memory.Reduced (Typ.Memory.Reduced s)
+end
+
+theorem Reduced.not_alias : ∀ s, ¬ Reduced (Typ.alias s) :=
+  fun _ => fun h => nomatch h
+
+def isScalar : Typ → Bool
+  | .prim .int => true
+  | .prim .bool => true
+  | .void => true
+  | _ => false
+
+def isSmall : Typ → Bool
+  | .mem (.struct _) => false
+  | _ => true
+
+def sizeof : Typ → Option Nat
+  | .prim .int => some 4
+  | .prim .bool => some 1
+  | .mem (.pointer _) => some 8
+  | .mem (.array _) => some 8
+  | .mem (.struct _) => none
+  | _ => none
