C0deine/utils/Symbol.lean
@@ -4,7 +4,8 @@ namespace C0deine
 
 structure Symbol where
   name : String
-  id : Nat
+  id : UInt64
 deriving DecidableEq, Inhabited
 
 instance : ToString Symbol where toString | s => s.name
+instance : Hashable Symbol where hash | s => s.id
